# corona-ontology.ttl
# RDFS Definitions for the "Corona" OT Performance Metrics Standard (Draft)

@prefix rdf: <http://www.w3.org/1999/02/22-rdf-syntax-ns#> .
@prefix rdfs: <http://www.w3.org/2000/01/rdf-schema#> .
@prefix xsd: <http://www.w3.org/2001/XMLSchema#> .
@prefix corona: <http://example.org/standards/corona/metrics#> .

# --- Base Classes ---

corona:PerformanceMetric rdf:type rdfs:Class ;
    rdfs:label "Performance Metric"@en ;
    rdfs:comment "The abstract concept of a performance metric for Operational Technology systems."@en .

corona:SampledMetric rdf:type rdfs:Class ;
    rdfs:subClassOf corona:PerformanceMetric ;
    rdfs:label "Sampled Metric"@en ;
    rdfs:comment "A performance metric observed over a specific time interval."@en .

corona:LifetimeMetric rdf:type rdfs:Class ;
    rdfs:subClassOf corona:PerformanceMetric ;
    rdfs:label "Lifetime Metric"@en ;
    rdfs:comment "A performance metric that accumulates over the lifetime of the system."@en .

corona:NetworkInterfaceMetric rdf:type rdfs:Class ;
    rdfs:subClassOf corona:PerformanceMetric ;
    rdfs:label "Network Interface Metric"@en ;
    rdfs:comment "A performance metric primarily associated with a network interface's activity."@en .

corona:ApplicationMetric rdf:type rdfs:Class ;
    rdfs:subClassOf corona:PerformanceMetric ;
    rdfs:label "Application Metric"@en ;
    rdfs:comment "A performance metric primarily associated with application-level interactions or protocol behavior."@en .

# --- Observation Node Property ---

corona:observedFrom rdf:type rdf:Property ;
    rdfs:label "Observed From"@en ;
    rdfs:comment "Specifies the node in the network from which the metric is observed."@en ;
    rdfs:domain corona:PerformanceMetric ;
    rdfs:range rdfs:Resource ; # Can point to any network node or resource
    rdfs:isDefinedBy corona: .

# --- Network Interface Metric Properties ---

corona:bytesReceived rdf:type rdf:Property ;
    rdfs:subPropertyOf corona:NetworkInterfaceMetric ;
    rdfs:label "Bytes Received"@en ;
    rdfs:comment "Total number of octets (bytes) received on an interface since the last counter reset or initialization. Wraparound behavior is implementation-defined."@en ;
    rdfs:range xsd:unsignedLong ;
    rdfs:isDefinedBy corona: .

corona:bytesSent rdf:type rdf:Property ;
    rdfs:subPropertyOf corona:NetworkInterfaceMetric ;
    rdfs:label "Bytes Sent"@en ;
    rdfs:comment "Total number of octets (bytes) sent from an interface since the last counter reset or initialization. Wraparound behavior is implementation-defined."@en ;
    rdfs:range xsd:unsignedLong ;
    rdfs:isDefinedBy corona: .

corona:packetsReceived rdf:type rdf:Property ;
    rdfs:subPropertyOf corona:NetworkInterfaceMetric ;
    rdfs:label "Packets Received"@en ;
    rdfs:comment "Total number of network packets (frames) received on an interface, including errored packets."@en ;
    rdfs:range xsd:unsignedLong ;
    rdfs:isDefinedBy corona: .

corona:packetsSent rdf:type rdf:Property ;
    rdfs:subPropertyOf corona:NetworkInterfaceMetric ;
    rdfs:label "Packets Sent"@en ;
    rdfs:comment "Total number of network packets (frames) transmitted from an interface."@en ;
    rdfs:range xsd:unsignedLong ;
    rdfs:isDefinedBy corona: .

corona:broadcastPacketsReceived rdf:type rdf:Property ;
    rdfs:subPropertyOf corona:NetworkInterfaceMetric ;
    rdfs:label "Broadcast Packets Received"@en ;
    rdfs:comment "Total number of broadcast packets received on an interface."@en ;
    rdfs:range xsd:unsignedLong ;
    rdfs:isDefinedBy corona: .

corona:errorPacketsReceived rdf:type rdf:Property ;
    rdfs:subPropertyOf corona:NetworkInterfaceMetric ;
    rdfs:label "Error Packets Received"@en ;
    rdfs:comment "Total number of inbound packets received with errors (e.g., CRC errors, framing errors)."@en ;
    rdfs:range xsd:unsignedLong ;
    rdfs:isDefinedBy corona: .

corona:packetsDroppedReceived rdf:type rdf:Property ;
    rdfs:subPropertyOf corona:NetworkInterfaceMetric ;
    rdfs:label "Packets Dropped Received"@en ;
    rdfs:comment "Total number of inbound packets discarded, e.g., due to buffer overflows or lack of resources."@en ;
    rdfs:range xsd:unsignedLong ;
    rdfs:isDefinedBy corona: .

corona:networkUtilization rdf:type rdf:Property ;
    rdfs:subPropertyOf corona:NetworkInterfaceMetric ;
    rdfs:label "Network Utilization"@en ;
    rdfs:comment "The percentage of available bandwidth currently being used on the network interface, typically calculated over a recent interval."@en ;
    rdfs:range xsd:float ; # Value between 0.0 and 100.0
    rdfs:isDefinedBy corona: .

corona:linkSpeed rdf:type rdf:Property ;
	rdfs:subPropertyOf corona:NetworkInterfaceMetric ;
	rdfs:label "Link Speed"@en ;
	rdfs:comment "The configured or negotiated speed of the network link. Units should be specified separately (e.g., Mbps)."@en ;
	rdfs:range xsd:unsignedInt ;
	rdfs:isDefinedBy corona: .


# --- Application Metric Properties ---

corona:readCommandLatency rdf:type rdf:Property ;
    rdfs:subPropertyOf corona:SampledMetric ;
    rdfs:label "Read Command Latency"@en ;
    rdfs:comment "Average time duration between sending a read request and receiving the corresponding response. Units should be specified separately, typically milliseconds."@en ;
    rdfs:range xsd:float ;
    rdfs:isDefinedBy corona: .

corona:writeCommandLatency rdf:type rdf:Property ;
    rdfs:subPropertyOf corona:SampledMetric ;
    rdfs:label "Write Command Latency"@en ;
    rdfs:comment "Average time duration between sending a write request and receiving the corresponding response or acknowledgment. Units should be specified separately, typically milliseconds."@en ;
    rdfs:range xsd:float ;
    rdfs:isDefinedBy corona: .

corona:requestSuccessPercentage rdf:type rdf:Property ;
    rdfs:subPropertyOf corona:ApplicationMetric ;
    rdfs:label "Request Success Percentage"@en ;
    rdfs:comment "The percentage of successful request-response transactions over a defined measurement interval. Calculation details (e.g., timeout criteria) are implementation-defined."@en ;
    rdfs:range xsd:float ; # Value between 0.0 and 100.0
    rdfs:isDefinedBy corona: .

corona:totalRequests rdf:type rdf:Property ;
    rdfs:subPropertyOf corona:LifetimeMetric ;
    rdfs:label "Total Requests"@en ;
    rdfs:comment "Total number of requests sent within the measurement interval for calculating success percentage."@en ;
    rdfs:range xsd:unsignedLong ;
    rdfs:isDefinedBy corona: .

corona:successfulResponses rdf:type rdf:Property ;
    rdfs:subPropertyOf corona:LifetimeMetric ;
    rdfs:label "Successful Responses"@en ;
    rdfs:comment "Total number of successful responses received within the measurement interval for calculating success percentage."@en ;
    rdfs:range xsd:unsignedLong ;
    rdfs:isDefinedBy corona: .

# BACnet-specific Application Metrics

corona:readPropertyRequests rdf:type rdf:Property ;
    rdfs:subPropertyOf corona:LifetimeMetric ;
    rdfs:label "ReadProperty Requests"@en ;
    rdfs:comment "Total number of ReadProperty requests sent."@en ;
    rdfs:domain corona:ApplicationMetric ;
    rdfs:range xsd:unsignedLong ;
    rdfs:isDefinedBy corona: .

corona:readPropertyResponses rdf:type rdf:Property ;
    rdfs:subPropertyOf corona:LifetimeMetric ;
    rdfs:label "ReadProperty Responses"@en ;
    rdfs:comment "Total number of ReadProperty responses received."@en ;
    rdfs:domain corona:ApplicationMetric ;
    rdfs:range xsd:unsignedLong ;
    rdfs:isDefinedBy corona: .

corona:totalProperties a rdf:Property ;
    rdfs:label "Total Properties" ;
    rdfs:comment "Total number of properties available in the BACnet object." ;
    rdfs:domain corona:ApplicationMetric ;
    rdfs:range xsd:unsignedLong .

corona:whoIsRequestsSent rdf:type rdf:Property ;
    rdfs:subPropertyOf corona:LifetimeMetric ;
    rdfs:label "WhoIs Requests Sent"@en ;
    rdfs:comment "Total number of WhoIs requests sent."@en ;
    rdfs:domain corona:ApplicationMetric ;
    rdfs:range xsd:unsignedLong ;
    rdfs:isDefinedBy corona: .

corona:globalWhoIsRequestsSent a rdf:Property ;
    rdfs:label "Global WhoIs Requests Sent" ;
    rdfs:comment "Number of global WhoIs requests sent." ;
    rdfs:domain corona:ApplicationMetric ;
    rdfs:range xsd:unsignedLong .

corona:directedWhoIsRequestsSent a rdf:Property ;
    rdfs:label "Directed WhoIs Requests Sent" ;
    rdfs:comment "Number of directed WhoIs requests sent." ;
    rdfs:domain corona:ApplicationMetric ;
    rdfs:range xsd:unsignedLong .

corona:iAmResponsesSent rdf:type rdf:Property ;
    rdfs:subPropertyOf corona:LifetimeMetric ;
    rdfs:label "IAm Responses Sent"@en ;
    rdfs:comment "Total number of IAm responses sent."@en ;
    rdfs:domain corona:ApplicationMetric ;
    rdfs:range xsd:unsignedLong ;
    rdfs:isDefinedBy corona: .

corona:iAmResponsesReceived a rdf:Property;
    rdfs:label "IAm Responses Received";
    rdfs:comment "Total number of IAm responses received.";
    rdfs:domain corona:ApplicationMetric;
    rdfs:range xsd:unsignedLong .

# --- Additional Network Interface Metrics ---

corona:broadcastPacketsSent rdf:type rdf:Property ;
    rdfs:subPropertyOf corona:NetworkInterfaceMetric ;
    rdfs:label "Broadcast Packets Sent"@en ;
    rdfs:comment "Total number of broadcast packets sent from an interface."@en ;
    rdfs:range xsd:unsignedLong ;
    rdfs:isDefinedBy corona: .

corona:broadcastRelayed rdf:type rdf:Property ;
    rdfs:subPropertyOf corona:NetworkInterfaceMetric ;
    rdfs:label "Broadcast Packets Relayed"@en ;
    rdfs:comment "Total number of broadcast packets relayed by this device (acting as a router or gateway)."@en ;
    rdfs:range xsd:unsignedLong ;
    rdfs:isDefinedBy corona: .

# --- Additional BACnet Application Metrics ---

corona:whoIsRequestsReceived rdf:type rdf:Property ;
    rdfs:subPropertyOf corona:LifetimeMetric ;
    rdfs:label "WhoIs Requests Received"@en ;
    rdfs:comment "Total number of WhoIs requests received."@en ;
    rdfs:domain corona:ApplicationMetric ;
    rdfs:range xsd:unsignedLong ;
    rdfs:isDefinedBy corona: .

corona:readPropertyRequestsSent rdf:type rdf:Property ;
    rdfs:subPropertyOf corona:LifetimeMetric ;
    rdfs:label "ReadProperty Requests Sent"@en ;
    rdfs:comment "Total number of ReadProperty requests sent."@en ;
    rdfs:domain corona:ApplicationMetric ;
    rdfs:range xsd:unsignedLong ;
    rdfs:isDefinedBy corona: .

corona:readPropertyRequestsReceived rdf:type rdf:Property ;
    rdfs:subPropertyOf corona:LifetimeMetric ;
    rdfs:label "ReadProperty Requests Received"@en ;
    rdfs:comment "Total number of ReadProperty requests received."@en ;
    rdfs:domain corona:ApplicationMetric ;
    rdfs:range xsd:unsignedLong ;
    rdfs:isDefinedBy corona: .

corona:readPropertyResponsesSent rdf:type rdf:Property ;
    rdfs:subPropertyOf corona:LifetimeMetric ;
    rdfs:label "ReadProperty Responses Sent"@en ;
    rdfs:comment "Total number of ReadProperty responses sent."@en ;
    rdfs:domain corona:ApplicationMetric ;
    rdfs:range xsd:unsignedLong ;
    rdfs:isDefinedBy corona: .

corona:readPropertyResponsesReceived rdf:type rdf:Property ;
    rdfs:subPropertyOf corona:LifetimeMetric ;
    rdfs:label "ReadProperty Responses Received"@en ;
    rdfs:comment "Total number of ReadProperty responses received."@en ;
    rdfs:domain corona:ApplicationMetric ;
    rdfs:range xsd:unsignedLong ;
    rdfs:isDefinedBy corona: .

# --- BACnet Router Metrics ---

corona:routedMessagesSent rdf:type rdf:Property ;
    rdfs:subPropertyOf corona:LifetimeMetric ;
    rdfs:label "Routed Messages Sent"@en ;
    rdfs:comment "Total number of messages routed and sent to other networks."@en ;
    rdfs:domain corona:ApplicationMetric ;
    rdfs:range xsd:unsignedLong ;
    rdfs:isDefinedBy corona: .

corona:routedMessagesReceived rdf:type rdf:Property ;
    rdfs:subPropertyOf corona:LifetimeMetric ;
    rdfs:label "Routed Messages Received"@en ;
    rdfs:comment "Total number of messages received that were routed from other networks."@en ;
    rdfs:domain corona:ApplicationMetric ;
    rdfs:range xsd:unsignedLong ;
    rdfs:isDefinedBy corona: .

corona:routedVia rdf:type rdf:Property ;
    rdfs:label "Routed Via"@en ;
    rdfs:comment "Identifies the router or gateway device through which this message was routed."@en ;
    rdfs:domain corona:ApplicationMetric ;
    rdfs:range rdfs:Resource ; # Points to another device URI
    rdfs:isDefinedBy corona: .

corona:routedDevicesSeen rdf:type rdf:Property ;
    rdfs:subPropertyOf corona:LifetimeMetric ;
    rdfs:label "Routed Devices Seen"@en ;
    rdfs:comment "Number of unique devices on other networks that have been seen through routing."@en ;
    rdfs:domain corona:ApplicationMetric ;
    rdfs:range xsd:unsignedLong ;
    rdfs:isDefinedBy corona: .